proof/correctness/Correctness_Conditions.ec
@@ -6,43 +6,67 @@ require import XMSS_IMPL.
 
 (* CPU FLAGS : of, cf, sf, pf, zf *)
 
-lemma test_8_bool (b1 b2 : bool) :  
-  (! (TEST_8 (SETcc b1) (SETcc b2)).`5) = ( b1 /\ b2 ).
-proof.
-rewrite /SETcc /TEST_8.
-case b1 => [| /#].
-case b2; move => ? ? => //=; smt(@W8). 
-qed.
+require import Array11.
 
-lemma cmp_W64 :
-    forall (a b : W64.t), (! (CMP_64 a b).`2) = (b \ule a).
-move => a b.
-case (b \ule a); by move => ? ; rewrite /CMP_64 /rflags_of_aluop //= #smt:(@W64).
-qed.
+lemma setcc_false (p : bool) : !p => SETcc p = W8.zero by rewrite /SETcc /#.
+lemma setcc_true  (p : bool) :  p => SETcc p = W8.one  by rewrite /SETcc /#.
 
 lemma cmp_eq_W32 :
     forall (a b : W32.t), (CMP_32 a b).`5 = (a = b).
 proof.
 move => a b.
-case (a = b); move => ?; rewrite /CMP_32 /rflags_of_aluop //= #smt:(@W32).
+case (a = b) => ?; rewrite /CMP_32 /rflags_of_aluop //=. 
+  + have ->:  (a - b) = W32.zero by smt(@W32).
+    smt().
+smt(@W32).
 qed.
 
-lemma test_cmp_32_64 (_a _b : W64.t) (_c _d : W32.t) :
-    (! (TEST_8 (SETcc (! (CMP_64 _a _b).`2)) (SETcc (CMP_32 _c _d).`5)).`5) = ((_b \ule _a) /\ _c = _d).
+lemma cmp_eq_W64 :
+    forall (a b : W64.t), (CMP_64 a b).`5 = (a = b).
 proof.
-rewrite cmp_eq_W32 cmp_W64.
-apply test_8_bool.
+move => a b.
+case (a = b) => ?; rewrite /CMP_64 /rflags_of_aluop //=. 
+  + have ->:  (a - b) = W64.zero by smt(@W64).
+    smt().
+smt(@W64).
 qed.
 
-(* cond = a >= b /\ c == d *)
-(* cond = b <= a /\ c = d *)
-lemma cond_u64_geq_u64_u32_eq_u32(_a : W64.t, _b : W64.t, _c : W32.t, _d :W32.t) :
-    hoare[M(Syscall).__cond_u64_geq_u64_u32_eq_u32 :
-      arg = (_a, _b, _c, _d) ==>
-        res = ( _b \ule _a /\ _c = _d )].
+lemma cmp_lt_W64 :
+    forall (a b : W64.t), (CMP_64 a b).`2 = (a \ult b).
+proof.
+move => a b.
+rewrite /CMP_64 /rflags_of_aluop => />; smt(@W64).
+qed.
+
+lemma treehash_cond_ll : islossless M(Syscall).__treehash_cond by proc; auto.
+
+pred treehash_cond (h : W32.t Array11.t) (o : W64.t) = 2 <= to_uint o /\ (h.[to_uint o - 2] = h.[to_uint o -1]).
+
+lemma treehash_cond_correct (h : W32.t Array11.t) (o : W64.t) : 
+    hoare [
+      M(Syscall).__treehash_cond :
+      0 <= to_uint o <= W32.max_uint /\
+      arg = (h, o) 
+      ==>
+      if treehash_cond h o then res = W8.one else res = W8.zero 
+    ].
 proof.
 proc.
-auto => />.
-rewrite /_uGE /_EQ /_uLT /_NEQ /_EQ #smt:(test_cmp_32_64).
+seq 3 : (#pre /\ bc1 = if (2 <= to_uint offset) then W8.one else W8.zero).
+  + auto => /> *.
+    case (2 <= to_uint o) => H; [rewrite setcc_true | rewrite setcc_false] => //; rewrite cmp_eq_W64 cmp_lt_W64 /_uGE /_uLT; [smt(@W64) |].
+    rewrite ultE of_uintK // #smt(@W64).
+if; first by auto => />.
+auto => /> *.
+split => *; [rewrite setcc_true | rewrite setcc_false ] => //; rewrite cmp_eq_W32 /_EQ !to_uintB 3:/#; by rewrite uleE /#.        
 qed.
 
+(* Same as previous lemma but this one is phoare *)
+lemma treehash_cond_correct_p (h : W32.t Array11.t) (o : W64.t) : 
+    phoare [
+      M(Syscall).__treehash_cond :
+      0 <= to_uint o <= W32.max_uint /\
+      arg = (h, o) 
+      ==>
+      if treehash_cond h o then res = W8.one else res = W8.zero 
+    ] =1%r by conseq treehash_cond_ll (treehash_cond_correct h o).
