proof/common/Array131.ec
@@ -1,0 +1,3 @@
+from Jasmin require import JArray.
+
+clone export PolyArray as Array131  with op size <- 131.
