proof/correctness/TreehashProof.ec
@@ -13,48 +13,36 @@ require import Params XMSS_MT_Params Types Address BaseW WOTS LTree XMSS_MT_Tree
 require import XMSS_IMPL Parameters.
 require import Repr2 Utils2.
 
-require import Array8 Array11 Array32 Array132 Array320 Array352 Array2144 Array2464.
+require import Array4 Array8 Array11 Array32 Array131 Array320 Array352 Array2144 Array2464.
 
 require import Correctness_Address.
 
+require import WArray32.
 
-(* stack u8[(XMSS_TREE_HEIGHT + 1) * XMSS_N] _stack; 
-   idx = 0;
-    while (idx < (1 << XMSS_TREE_HEIGHT))
+(* 
+{1} => proc __treehash (root:W8.t Array32.t, sk_seed:W8.t Array32.t,
+                   pub_seed:W8.t Array32.t, start_index:W32.t,
+                   target_height:W32.t, subtree_addr:W32.t Array8.t)
+
+{2} => proc treehash(pub_seed sk_seed : seed, s t : int, address : adrs) : nbytes
 *)
-
-(* _stack{1} = W8.t Array352.t *)
-(* For this proof, the address will be the zero address *)
-
-
-
-(* arg{1}
-
-root:W8.t Array32.t
-sk_seed:W8.t Array32.t,
-pub_seed:W8.t Array32.t, 
-s:W32.t, 
-target_height:W32.t,
-subtree_addr:W32.t Array8.t
-
-*)
-
-(* This only works for kg because of  arg{2}.`3 = 0 /\ arg{2}.`4 = h *)
 lemma treehash_correct ( _sk_seed _pub_seed : W8.t Array32.t, _s _t:W32.t, _addr:W32.t Array8.t): 
     n = XMSS_N /\
     d = XMSS_D /\
-    h = XMSS_FULL_HEIGHT =>
+    h = XMSS_TREE_HEIGHT =>
     equiv [
       M(Syscall).__treehash ~ TreeHash.treehash :
+
       arg{1}.`2 = _sk_seed /\
       arg{1}.`3 = _pub_seed /\
       arg{1}.`4 = _s /\
       arg{1}.`5 = _t /\
       arg{1}.`6 = _addr /\
+      
       arg{2}.`1 = NBytes.insubd (to_list _pub_seed) /\
       arg{2}.`2 = NBytes.insubd (to_list _sk_seed) /\
-      arg{2}.`3 = 0 /\
-      arg{2}.`4 = h /\
+      arg{2}.`3 = to_uint _s /\
+      arg{2}.`4 = to_uint _t /\
       arg{2}.`5 = _addr /\
 
       0 <= to_uint _t <= XMSS_TREE_HEIGHT
@@ -62,85 +50,86 @@ lemma treehash_correct ( _sk_seed _pub_seed : W8.t Array32.t, _s _t:W32.t, _addr
       to_list res{1} = val res{2}
     ].
 proof.
-rewrite /XMSS_N /XMSS_D /XMSS_FULL_HEIGHT => [#] n_val d_val h_val.
+rewrite /XMSS_N /XMSS_D /XMSS_TREE_HEIGHT => [#] n_val d_val treeheight_val.
 proc => /=.
-seq 7 0 : #pre; first by auto.
-seq 0 1 : (#pre /\ size stack{2} = h + 1); first by auto => />; rewrite size_nseq #smt:(ge0_h ge0_d). 
-seq 1 1 : (#pre /\ to_uint offset{1} = offset{2}); first by auto. 
-seq 1 0 : (#pre /\ ots_addr{1}= zero_addr).
-  + inline {1} 1; wp.
-    ecall {1} (zero_addr_res ots_addr{1}).
-    auto.
-seq 1 0 : (#pre /\ ltree_addr{1}= zero_addr).
-  + inline {1} 1; wp.
-    ecall {1} (zero_addr_res ots_addr{1}).
-    auto.
-seq 1 0 : (#pre /\ node_addr{1}= zero_addr).
-  + inline {1} 1; wp.
-    ecall {1} (zero_addr_res ots_addr{1}).
-    auto.
 
-seq 11 3 : (sub _stack{1} 0 32 = val node{2}); last first.
-  + while {1} 
-    (#pre /\ 0 <= j{1} <= 32 /\
-     forall (k : int), 0 <= k < j{1} => root{1}.[k] = _stack{1}.[k])
-    (32 - j{1}); last first.
-       * auto => /> &1 &2 <-.
-         split => [/# | jL rootL].
-         split => [/# | ???].
-         have ->: jL = 32 by smt().
-         move => H1.
-         apply (eq_from_nth witness); first by rewrite size_sub // size_to_list.
-         rewrite size_to_list => i?.
-         rewrite get_to_list nth_sub // /#.
-       * auto => /> &hr *.
-         do split; 1,2,4: by smt().
-         move => k??.
-         rewrite get_setE /#. 
+swap {2} 3 -2.
+seq 8 1: (#pre /\ offset{1} = W64.zero /\ offset{2} = 0); first by auto.
 
-seq 7 0 : (true). (* set appropriate condition *)
-      + inline {1}.
-        auto => />.
+seq 11 4 : (sub _stack{1} 0 n = val (nth witness stack{2} 0)); last first.
+  + while {1}
+    (0 <= j{1} <= 32 /\
+     forall (k : int), 0 <= k < j{1} => root{1}.[k] = nth witness (val (nth witness stack{2} 0)) k)
+    (32 - j{1}); first by auto => />; admit. (* /#. *)
+    auto => /> &1 &2 ?; split => [/# |].
+    move => j ?; split => [/# |???].
+    have ->: j = 32 by smt().
+    move => H.
+    apply (eq_from_nth witness); first by rewrite valP n_val size_to_list.
+    rewrite size_to_list => ??.
+    by rewrite get_to_list H.
+
+seq 1 0 : (#pre /\ ots_addr{1} = subtree_addr{1}).
+      + auto => /> ??.
+        rewrite tP => j?.
+        rewrite initiE //= get32E pack4E wordP => i?.
+        rewrite initiE //= initiE 1:/# /= /init64 initiE 1:/# /= /copy_64 initiE 1:/# /=.
+(*
+        rewrite  get64E pack8E bits8iE 1:/# initiE 1:/# /= initiE 1:/# //= /init32 initiE 1:/# /= /#.
+
+seq 1 0 : (#pre /\ ltree_addr{1} = subtree_addr{1}).
+      + auto => /> ??.
+        rewrite tP => j?.
+        rewrite initiE //= get32E pack4E wordP => i?.
+        rewrite initiE //= initiE 1:/# /= /init64 initiE 1:/# /= /copy_64 initiE 1:/# /=.
+        rewrite  get64E pack8E bits8iE 1:/# initiE 1:/# /= initiE 1:/# //= /init32 initiE 1:/# /= /#.
+
+seq 1 0 : (#pre /\ node_addr{1} = subtree_addr{1}).
+      + auto => /> ??.
+        rewrite tP => j?.
+        rewrite initiE //= get32E pack4E wordP => i?.
+        rewrite initiE //= initiE 1:/# /= /init64 initiE 1:/# /= /copy_64 initiE 1:/# /=.
+        rewrite  get64E pack8E bits8iE 1:/# initiE 1:/# /= initiE 1:/# //= /init32 initiE 1:/# /= /#.
+
+
+seq 0 2 : (#pre /\ size stack{2} = (h %/d + 1) /\ size heights{2} = (h %/ d)).
+      + auto => /> *; rewrite size_nseq /#.
+
+seq 4 0 : (
+      #{/~ ots_addr{1} = subtree_addr{1}}
+       {/~ ltree_addr{1} = subtree_addr{1}}
+       {/~ node_addr{1} = subtree_addr{1}}pre /\
+      ots_addr{1} = set_type subtree_addr{1} 0 /\
+      ltree_addr{1} = set_type subtree_addr{1} 1 /\
+      node_addr{1} = set_type subtree_addr{1} 2
+); first by inline; auto.
 
 swap {1} 1 2.
-seq 2 0 : (#pre /\ to_uint upper_bound{1} = 2 ^ t{2}).
-      + auto => /> &1 &2.
-        rewrite (: 31 = 2^5 - 1) 1:/# and_mod //.
-        have ->: truncateu8 ((of_int (to_uint target_height{1} %% 2 ^ 5)))%W32 = 
-                 W8.of_int t{2} by admit.
-        search (`<<`).
-        rewrite shl_shlw.
-          * admit.
-        admit.
 
-
-seq 2 2: (sub _stack{1} 0 32 = val (nth witness stack{2} (offset{2} - 1))); last by auto.
+seq 2 0 : (#pre /\ to_uint upper_bound{1} = 2^t{2}).
+    + auto => /> *.
+      rewrite (: 31 = 2^5 - 1) 1:/# and_mod // shl_shlw 1:#smt:(@W32) of_uintK to_uint_shl /#.
 
 while (
-          i{2} = to_uint i{1} /\
-          to_uint upper_bound{1} = t{2}
-); last first.
-    + auto => /> &1 &2 *.
-      admit.
+  0 <= i{2} <= 2^t{2} /\
+  to_uint i{1} = i{2} /\
+  to_uint upper_bound{1} = 2^t{2} /\
+  #post (* This is false *)
+).
 
-seq 2 0 : (#pre /\ t32{1} = s{1} + i{1}); first by auto.
-
-inline {1} M(Syscall).__gen_leaf_wots_ M(Syscall)._gen_leaf_wots M(Syscall).__gen_leaf_wots. (* Same as pkgen + ltree *)
-
+    + admit.
+    + admit.
+*)
 admit.
+admit.
+
 qed.
 
-(*
-
-arg{2}:
-pub_seed sk_seed : seed, idx : W32.t, address : adrs
-
- *)
 lemma build_auth_path_correct (_pub_seed _sk_seed : W8.t Array32.t, _idx : W32.t, a : adrs) :
     len = XMSS_WOTS_LEN /\ 
     n = XMSS_N /\
     d = XMSS_D /\
-    h = XMSS_FULL_HEIGHT =>
+    h = XMSS_TREE_HEIGHT =>
     equiv[
       M(Syscall).__build_auth_path ~ TreeSig.buildAuthPath :
       arg{1}.`2 = _sk_seed /\
@@ -153,13 +142,12 @@ lemma build_auth_path_correct (_pub_seed _sk_seed : W8.t Array32.t, _idx : W32.t
       arg{2}.`3 = _idx /\
       arg{2}.`4 = a /\
 
-
-      0 <= to_uint _idx < 2^XMSS_FULL_HEIGHT (* ou tree height *)
+      0 <= to_uint _idx < 2 ^ XMSS_TREE_HEIGHT
       ==>
       res{2} = EncodeAuthPath (to_list res{1})
     ].
 proof.
-rewrite /XMSS_WOTS_LEN /XMSS_N /XMSS_D /XMSS_FULL_HEIGHT => [#] len_val n_val d_val h_val.
+rewrite /XMSS_WOTS_LEN /XMSS_N /XMSS_D /XMSS_TREE_HEIGHT => [#] len_val n_val d_val h_val.
 proc => /=.
 seq 2 3 : (#pre /\ ={j} /\ j{1} = 0 /\ size authentication_path{2} = h). 
   + auto => />; by rewrite size_nseq h_val.
@@ -192,104 +180,137 @@ conseq (: _ ==>
           rewrite -(all_nthP P L witness) /P /L size_map H h_val => k?.
           by rewrite (nth_map witness) 1:/# valP.
     rewrite (nth_map witness) /#.
- 
-while ( 
-  0 <= to_uint idx{2} < 1024 /\
 
-  0 <= j{1} <= h /\ ={j} /\
-  size authentication_path{2} = h /\
-
-  idx{2} = i{1} /\
-  to_list sk_seed{1}  = val sk_seed{2} /\
+(* Rewrite #pre *)
+conseq ( :
+  to_list sk_seed{1} = val sk_seed{2} /\
   to_list pub_seed{1} = val pub_seed{2} /\
+  addr{1} = address{2} /\
+  ={j} /\ j{1} = 0 /\
+  i{1} = idx{2} /\ 0 <= to_uint idx{2} < 2 ^ XMSS_TREE_HEIGHT /\
+  size authentication_path{2} = 10
+  ==> _
+).
+    + auto => /> *; split.
+        * apply (eq_from_nth witness); first by rewrite valP size_to_list n_val.
+          rewrite size_to_list => j?.
+          by rewrite insubdK // /P size_to_list n_val.
+        * split => [| /#].
+          apply (eq_from_nth witness); first by rewrite valP size_to_list n_val.
+          rewrite size_to_list => j?.
+          by rewrite insubdK // /P size_to_list n_val.
+
+while (
+  0 <= to_uint idx{2} < 2 ^ XMSS_TREE_HEIGHT /\
+  to_list sk_seed{1} = val sk_seed{2} /\
+  to_list pub_seed{1} = val pub_seed{2} /\
+  addr{1} = address{2} /\
+  i{1} = idx{2} /\
+  ={j} /\ 0 <= j{2} <= 10 /\ 
+  size authentication_path{2} = 10 /\
+
+  (0 <= to_uint idx{2} < 2 ^ XMSS_TREE_HEIGHT) /\
 
   forall (k : int), 0 <= k < n * j{1} => auth_path{1}.[k] = nth witness (nbytes_flatten authentication_path{2}) k
 ); last first.
-    + auto => /> &2 *. 
-      do split; 1,4,5: by smt().
-        * by rewrite insubdK // /P size_to_list n_val.
-        * by rewrite insubdK // /P size_to_list n_val.
-        * move => authPathL authPathR j H0 H1 H2 H3 H4 ?? H5.
-          have j_val: j = h by smt().
-          clear H0 H1 H2 H3.
-          rewrite /EncodeAuthPath. 
-          apply (eq_from_nth witness); first by rewrite size_to_list size_nbytes_flatten_2 H4 n_val h_val.
-          rewrite size_to_list => i?.
-          by rewrite get_to_list H5 // n_val j_val h_val.
-seq 3 1 : (#pre /\ to_uint k{1} = k{2}); first by auto.
-seq 3 0 : (#pre /\ to_uint s{1} = k{2} * 2^j{1}).
-    + auto => /> &1 &2 *. 
-      rewrite shl_shlw 1:/# to_uint_shl 1:/#. 
-      admit.
+    + auto => /> &1 &2 ?????.
+      split => [/# | authL authR j ????H0].
+      have ->: j = h by smt().
+      rewrite n_val h_val /= => H1.
+      split => [| /#].
+      apply (eq_from_nth witness); first by rewrite size_to_list size_nbytes_flatten_2 H0 n_val.
+      rewrite size_to_list => ??.
+      by rewrite  get_to_list H1.
+
+
+seq 4 1 : (#pre /\ to_uint k{1} = k{2} * 2^j{1}).
+    + auto => /> &1 &2 ? H *.
+      rewrite /XMSS_TREE_HEIGHT /= in H.
+      rewrite shl_shlw 1:/# /(`>>`) of_uintK.
+      pose X := (idx{2} `>>>` j{2} %% W8.modulus %% 32).
+      admit. (* TODO: FIXME: *)
 
 seq 1 1 : (#pre /\ to_list node{1} = val t{2}).
-    + inline {1} M(Syscall).__treehash_ M(Syscall)._treehash.
-      wp.
-      exists * sk_seed1{1}, pub_seed1{1}, s1{1}, t0{1}, subtree_addr0{1}.
+    + inline {1} 1.
+      inline {1} 13.
+      wp; sp.
+      exists * pub_seed{1}, sk_seed{1}, k{1}, (of_int j{1})%W32, addr{1}.
       elim * => P0 P1 P2 P3 P4.
-      call {1} (treehash_correct P0 P1 P2 P3 P4) => [/# |].
-      auto => /> &1 &2 *. admit.
+      call {1} (treehash_correct P1 P0 P2 P3 P4) => [/# |].
+      skip => /> &1 &2 H0 H1 H2 H3 H4 H5 H6 H7 H8 H9 ->.
+      do split; 1,2:smt(@NBytes).
+         * rewrite of_uintK /#.
+         * rewrite of_uintK /#.
+         * smt(@W32 pow2_32).
 
-auto => /> &1 &2 ????H??H0???H1. 
-do split; 1,2,5,6: by smt().
-    * by rewrite size_put.
-move => k??.
-rewrite initiE 1:/# => />.
-rewrite /nbytes_flatten (nth_flatten witness n).
-   * pose P := (fun (s : W8.t list) => size s = n).
-     pose L := (map NBytes.val (put authentication_path{2} j{2} t{2})).
-     rewrite -(all_nthP P L witness) /P /L size_map size_put H h_val => j?.
-     by rewrite (nth_map witness) 1:#smt:(size_put) valP.
-rewrite (nth_map witness) 1:#smt:(size_put) nth_put 1:/#.
-case (j{2} * 32 <= k && k < j{2} * 32 + 32) => H2.
-   * rewrite ifT 1:/# -H1 get_to_list /#.
-   * rewrite ifF 1:/# H0 1:/# /nbytes_flatten (nth_flatten witness n).
-       - pose P := (fun (s0 : W8.t list) => size s0 = n).
-         pose L := (map NBytes.val authentication_path{2}).
-         rewrite -(all_nthP P L witness) /P /L size_map H h_val => j?.
-         by rewrite (nth_map witness) 1:/# valP.
-     by rewrite (nth_map witness) 1:/#.
-qed.
- 
+auto => /> &1 &2 H0 H1 H2 H3 H4 H5 H6 H7 H8 H9 H10 H11; do split; 1,2,5,6: by smt().
+    - by rewrite size_put.
+    - move => k??.
 
-lemma sub_sub_list (x : W8.t t) (k l : int) :
-    0 <= l /\ 0 <= k =>
-    sub x k l = sub_list (to_list x) k l.
-proof.
-move => [#] ??.
-apply (eq_from_nth witness); first by rewrite size_sub // size_sub_list.
-rewrite size_sub // => i?.
-by rewrite nth_sub // /sub_list nth_mkseq.
+rewrite initiE 1:/# /= /nbytes_flatten (nth_flatten witness 32).
+    + pose P := (fun (s : W8.t list) => size s = 32).
+      pose L := (map NBytes.val (put authentication_path{2} j{2} t{2})).
+      rewrite -(all_nthP P L witness) /P /L size_map size_put H6 => i?.
+      rewrite (nth_map witness); first by rewrite size_put /#.
+      by rewrite valP n_val.
+rewrite (nth_map witness); first by rewrite size_put /#.
+rewrite nth_put 1:/#.
+case (j{2} * 32 <= k && k < j{2} * 32 + 32) => ?.
+    + rewrite ifT 1:/# -H11 get_to_list /#.
+    + rewrite ifF 1:/# H7 1:/# /nbytes_flatten (nth_flatten witness 32).
+         - pose P := (fun (s : W8.t list) => size s = 32).
+           pose L := (map NBytes.val authentication_path{2}).
+           rewrite -(all_nthP P L witness) /P /L size_map => ??.
+           by rewrite (nth_map witness) 1:/# valP n_val.
+      by rewrite (nth_map witness) 1:/#.
 qed.
 
 
-lemma treesig_correct :
+lemma treesig_correct (_m : W8.t Array32.t, _sk : W8.t Array131.t, _idx_sig : W32.t, _addr : W32.t Array8.t) :
     n = XMSS_N /\
     len = XMSS_WOTS_LEN /\ 
     d = XMSS_D /\
-    h = XMSS_FULL_HEIGHT =>
+    h = XMSS_TREE_HEIGHT =>
     equiv [
       M(Syscall).__tree_sig ~ TreeSig.treesig:
-      true 
+      arg{1}.`2 = _m /\
+      arg{1}.`3 = _sk /\
+      arg{1}.`4 = _idx_sig /\
+      arg{1}.`5 = _addr /\
+
+      arg{2}.`1 = NBytes.insubd (to_list _m) /\
+      arg{2}.`2 = NBytes.insubd (to_list _sk)
+
       ==>
       res{2} = EncodeReducedSignature (to_list res{1}.`1)
     ].
 proof.
 rewrite /XMSS_N /XMSS_WOTS_LEN /XMSS_D /XMSS_FULL_HEIGHT => [#] n_val len_val d_val h_val.
 proc => /=.
-seq 4 0 : #pre; first by auto.
-seq 2 0 : (
-  #pre /\ 
+seq 6 0 : (
   to_list pub_seed{1} = sub sk{1} (4 + 3*32) 32 /\
   to_list sk_seed{1} = sub sk{1} 4 32
 ).
     + auto => /> *; split.
          * apply (eq_from_nth witness); first by rewrite size_to_list size_sub.
            rewrite size_to_list => i?.
-           by rewrite get_to_list initiE // nth_sub.
+           rewrite get_to_list initiE // nth_sub //.
          * apply (eq_from_nth witness); first by rewrite size_to_list size_sub.
            rewrite size_to_list => i?.
            by rewrite get_to_list initiE // nth_sub.
+
+seq 1 1 : (#pre /\ auth{2} = EncodeAuthPath (to_list auth_path{1})).
+    + exists * pub_seed{1}, sk_seed{1}, idx_sig{1}, addr{1}.
+      elim * => P0 P1 P2 P3.
+      call {1} (build_auth_path_correct P0 P1 P2 P3) => [/# |].
+      skip => /> *; do split.
+
+
+       
+
+
+
+
 
 conseq (: _ ==>
   sub sig{1} 0 (67*32)       = DecodeWotsSignature_List sig_ots{2} /\
